steel/Learn.Steel.List.Impl.fst
@@ -8,11 +8,13 @@ module U32 = FStar.UInt32
 open Steel.Effect
 open Steel.Effect.Atomic
 open Steel.Reference
+open Learn.Steel.Util
 
-open Learn.Steel.List.DataD
 open Learn.Steel.List.Data
 open Learn.Steel.List.Derived
 
+
+(* [length] *)
 
 let rec length (#a : Type) (r : ref (cell a))
   : Steel  U32.t
@@ -21,7 +23,7 @@ let rec length (#a : Type) (r : ref (cell a))
           (ensures  fun h0 len h1 -> frame_equalities (mlistN r) h0 h1 /\
                                   U32.v len = L.length (sel_listN r h0))
   =
-    let b  = listN_is_nil r in
+    let b = listN_is_nil r in
     if b
     then return 0ul
     else begin
@@ -31,6 +33,8 @@ let rec length (#a : Type) (r : ref (cell a))
       return U32.(len' +^ 1ul)
     end
 
+
+(* [insert] *)
 
 let rec insert_aux (#a : Type) (i : U32.t) (x : ref (cell a))
                    (entry : ref (cell a)) (len : G.erased nat) (exit : G.erased (ref (cell a)))
@@ -44,7 +48,7 @@ let rec insert_aux (#a : Type) (i : U32.t) (x : ref (cell a))
     (**) let len1 = G.hide (len - 1) in
     (**) mlist_rew_len entry len (len1+1) exit;
     let nxt = list_next entry len1 exit in
-    if U32.v i = 1
+    if i = 1ul
     then begin
       let x_c = read x in
       write x ({x_c with next = nxt});
@@ -78,7 +82,104 @@ let insert (#a : Type) (i : U32.t) (x : ref (cell a))
     end
 
 
+(* alternative version using aptr *)
+
+inline_for_extraction
+let insert2_ty (#a : Type) (i : U32.t) (x : ref (cell a)) (r : aptr (ref (cell a))) : Type =
+  (entry : G.erased (ref (cell a))) -> (len : G.erased nat) -> (exit : G.erased (ref (cell a))) ->
+  Steel (G.erased (ref (cell a)))
+        (vptr x `star` r.vp `star` mlist entry len exit)
+        (fun entry' -> r.vp `star` mlist entry' (len+1) exit)
+        (requires fun h0  -> U32.v i <= len /\
+                          aptr_val r h0 == G.reveal entry)
+        (ensures  fun h0 entry' h1 ->
+                          U32.v i <= len /\
+                          aptr_updt r entry' h0 h1 /\
+                          sel_list entry' (len+1) exit h1
+                            == Ll.insert (U32.v i) (x, (sel x h0).data) (sel_list entry len exit h0))
+
+inline_for_extraction noextract
+let insert2_body (#a : Type)
+  ($rec_f : (i:U32.t) -> (x : ref (cell a)) -> (r : ref (cell a)) ->
+            insert2_ty #a i x (aptr_of_get_set cell_gs_next r))
+  (i : U32.t) (x : ref (cell a)) (r : aptr (ref (cell a)))
+  : insert2_ty i x r
+  = fun g_entry len exit ->
+    let entry = r.read () in
+    (**) change_equal_slprop (mlist g_entry len exit) (mlist entry len exit);
+    if i = 0ul
+    then begin
+      let x_c = read x in
+      write x ({x_c with next = entry});
+      (**) intro_mlist_cons x entry len exit;
+      r.write x;
+      x
+    end else begin
+      (**) let len' = G.hide (len - 1)                            in
+      (**) mlist_rew_len entry len (len'+1) exit;
+      (**) let entry'0 = elim_mlist_cons entry len' exit          in
+      let entry' = rec_f U32.(i -^ 1ul) x entry entry'0 len' exit in
+      (**) intro_mlist_cons entry entry' (len'+1) exit;
+      (**) mlist_rew_len entry ((len'+1)+1) (len+1) exit;
+      entry
+    end
+
+let rec insert2_cell_gs_next (#a : Type) (i : U32.t) (x : ref (cell a)) (r : ref (cell a))
+                             (entry : G.erased (ref (cell a))) (len : G.erased nat) (exit : G.erased (ref (cell a)))
+                 
+  : Steel (G.erased (ref (cell a)))
+          (vptr x `star` (aptr_of_get_set cell_gs_next r).vp `star` mlist entry len exit)
+          (fun entry' -> (aptr_of_get_set cell_gs_next r).vp `star` mlist entry' (len+1) exit)
+          (requires fun h0  -> U32.v i <= len /\
+                            aptr_val (aptr_of_get_set cell_gs_next r) h0 == G.reveal entry)
+          (ensures  fun h0 entry' h1 ->
+                                U32.v i <= len /\
+                                aptr_updt (aptr_of_get_set cell_gs_next r) entry' h0 h1 /\
+                                sel_list entry' (len+1) exit h1
+                                == Ll.insert (U32.v i) (x, (sel x h0).data) (sel_list entry len exit h0))
+  = insert2_body #a (insert2_cell_gs_next #a) i x (aptr_of_get_set cell_gs_next r) entry len exit
+
+inline_for_extraction
+let insert2 (#a : Type) (i : U32.t) (x : ref (cell a)) (r : aptr (ref (cell a)))
+  : insert2_ty #a i x r
+  = insert2_body #a (insert2_cell_gs_next #a) i x r
+
+(* [reverse] *)
+
+let rec reverse_aux (#a : Type) (r_f r_r : ref (cell a))
+  : Steel (ref (cell a))
+          (mlistN r_f `star` mlistN r_r) (fun rt -> mlistN rt)
+          (requires fun _ -> True)
+          (ensures fun h0 rt h1 ->
+             sel_listN rt h1 == L.rev_acc (sel_listN r_f h0) (sel_listN r_r h0))
+  =
+    let b  = listN_is_nil r_f in
+    if b
+    then begin
+      (**) elim_mlistN_nil r_f;
+      return r_r
+    end else begin
+      let r_f' = listN_next r_f in
+      let x_c  = read r_f       in (* TODO? factorize with listN_next *)
+      write r_f ({x_c with next = r_r});
+      (**) intro_mlistN_cons r_f r_r;
+      reverse_aux r_f' r_f
+    end
+
+let reverse (#a : Type) (r : ref (cell a))
+  : Steel (ref (cell a))
+          (mlistN r) (fun rt -> mlistN rt)
+          (requires fun _ -> True)
+          (ensures fun h0 rt h1 ->
+            sel_listN rt h1 == L.rev (sel_listN r h0))
+  =
+    (**) intro_mlistN_nil null;
+    reverse_aux r null
+
 (* ----------------- *)
 
-let length_u32 = length #U32.t
-let insert_u32 = insert #U32.t
+let length_u32  = length  #U32.t
+let insert_u32  = insert  #U32.t
+let insert2_u32 (i : U32.t) (x : ref (cell U32.t)) (r : ref (ref (cell U32.t))) =
+  insert2 #U32.t i x (aptr_of_vptr r)
+let reverse_u32 = reverse #U32.t
