steel/Learn.Steel.fst
@@ -33,3 +33,107 @@ let alloc_test () : Steel unit emp (fun () -> emp) (fun _ -> True) (fun _ () _ -
     let x = read r in
     (**) assert (x == 1ul);
     free r
+
+
+(* -------------------------- *)
+
+inline_for_extraction noextract noeq
+type aptr_p' (t : Type) = {
+  a  : Type;
+  vp : a -> vprop;
+  of_sel  : (r:a) -> normal (t_of (vp r)) -> GTot t;
+  set_sel : (r:a) -> normal (t_of (vp r)) -> (x : t) ->
+            Ghost (normal (t_of (vp r))) (requires True) (ensures fun rt -> of_sel r rt == x);
+  read  : (r:a) -> Steel t (vp r) (fun _ -> vp r) (requires fun _ -> True)
+                     (ensures fun h0 x h1 -> frame_equalities (vp r) h0 h1 /\ x == of_sel r (h0 (vp r)));
+  write : (r:a) -> (x : t) -> Steel unit (vp r) (fun _ -> vp r) (requires fun _ -> True)
+                     (ensures fun h0 () h1 -> h1 (vp r) == set_sel r (h0 (vp r)) x)
+}
+
+inline_for_extraction noextract
+type aptr_p (t : Type) = p:aptr_p' t {
+     forall (r:p.a) (s : normal (t_of (p.vp r))) (x0 x1 : t) . {:pattern (p.set_sel r (p.set_sel r s x0) x1)}
+       p.set_sel r (p.set_sel r s x0) x1 == p.set_sel r s x1
+  }  (* TODO [set_sel s (of_sel s) == s] *)
+
+
+inline_for_extraction noextract noeq
+type get_set_t' (c t : Type) = {
+  get : c -> Tot t;
+  set : c -> t -> Tot c;
+}
+
+inline_for_extraction noextract
+type get_set_t (c t : Type) = p:get_set_t' c t {
+     (forall (s : c) (x : t) . {:pattern (p.get (p.set s x))}
+        p.get (p.set s x) == x) /\
+     (forall (s : c) (x0 x1 : t) . {:pattern (p.set (p.set s x0) x1)}
+        p.set (p.set s x0) x1 == p.set s x1)
+  }
+
+inline_for_extraction noextract
+let aptr_of_vptr (#t : Type) : Tot (aptr_p t) = {
+  a       = ref t;
+  vp      = vptr;
+  of_sel  = (fun r x   -> (x <: t));
+  set_sel = (fun r _ x -> x);
+  read    = (fun r   -> read r);
+  write   = (fun r x -> write r x)
+}
+
+inline_for_extraction noextract
+let aptr_of_get_set (#c #t : Type) ($p : get_set_t c t) : Tot (aptr_p t) = {
+  a       = ref c;
+  vp      = vptr;
+  of_sel  = (fun r x   -> p.get x);
+  set_sel = (fun r s x -> p.set s x);
+  read    = (fun r   -> let s = read r in p.get s);
+  write   = (fun r x -> let s = read r in write r (p.set s x))
+}
+
+
+inline_for_extraction noextract
+let test_set_ptr (xp yp : aptr_p U32.t) (x : xp.a) (y : yp.a)
+  : Steel unit (xp.vp x `star` yp.vp y) (fun () -> xp.vp x `star` yp.vp y)
+               (requires fun _ -> True)
+               (ensures fun h0 () h1 -> h1 (xp.vp x) == h0 (xp.vp x) /\
+                                     h1 (yp.vp y) == yp.set_sel y (h0 (yp.vp y)) (xp.of_sel x (h0 (xp.vp x))))
+  = let v = xp.read x in
+    yp.write y v
+
+(*
+inline_for_extraction noextract
+let rec test_set_ptr_rec (i : U32.t) (x y : aptr_t U32.t)
+  : Steel unit (x.vp `star` y.vp) (fun () -> x.vp `star` y.vp)
+               (requires fun _ -> True)
+               (ensures fun h0 () h1 -> h1 x.vp == h0 x.vp /\
+                                     h1 y.vp == y.set_sel (h0 y.vp) (x.of_sel (h0 x.vp)))
+  = if i = 0ul then begin
+      let v = x.read () in
+      y.write v
+    end else
+      test_set_ptr_rec U32.(i -^ 1ul) x y
+*)
+
+type test_struct = {
+  fld_a : U32.t;
+  fld_b : bool
+}
+
+inline_for_extraction noextract
+let test_struct_gs_fld_a : get_set_t test_struct U32.t = {
+  get = (fun c -> c.fld_a);
+  set = (fun c x -> {c with fld_a = x})
+}
+
+let test_set_ptr_caller () : SteelT unit emp (fun () -> emp)
+  =
+    let x  = malloc #U32.t 42ul in
+    let ys = malloc #test_struct ({fld_a = 0ul; fld_b = false}) in
+    test_set_ptr aptr_of_vptr (aptr_of_get_set test_struct_gs_fld_a) x ys;
+    let i = read x in
+      assert (i == 42ul);
+    let i = read ys in
+      assert (i == {fld_a = 42ul; fld_b = false});
+    free x;
+    free ys
